#+title: Lösungen zum 4. Übungsblatt
#+date: 2017-11-08
#+email: tobias.denkinger@tu-dresden.de
#+options: toc:nil \n:yes

* Lösung zu Aufgabe 2.2.39
** Teilaufgabe a

#+begin_src
f(ρ) = S:⎛ ⟦[B]b⟧(ρ)⎞ = ⎛ (ρ(B) ∪ {ε}) ⋅ {b} ⎞ = ⎛ ρ(B) ⋅ {b} ∪ {b} ⎞
       B:⎝ ⟦Sb⟧(ρ)  ⎠   ⎝ ρ(S) ⋅ {b}         ⎠   ⎝ ρ(S) ⋅ {b}       ⎠

⊥ = ⎛ ∅ ⎞
    ⎝ ∅ ⎠
  ↦ ⎛ {b} ⎞
    ⎝ ∅   ⎠
  ↦ ⎛ {b}  ⎞
    ⎝ {bb} ⎠
  ↦ ⎛ {b, bbb} ⎞
    ⎝ {bb}     ⎠
  ↦ ⎛ {b, bbb}   ⎞
    ⎝ {bb, bbbb} ⎠
  ↦ ⎛ {b¹, b³, b⁵} ⎞
    ⎝ {b², b⁴}     ⎠
#+end_src

** Teilaufgabe b

  * W(ℰ, S) = { b(bb)ⁱ | i ∈ ℕ }
  * W(ℰ, B) = { bb(bb)ⁱ | i ∈ ℕ}

** Teilaufgabe c

Seien ρ(S) = ρ(A) = { (ba)ⁿb ∣ n ∈ ℕ }.  Zu zeigen: ⟦{ba}A⟧(ρ) = ρ(S).

Beweis:

⟦{ba}A⟧(ρ)
= ⟦{ba}⟧(ρ) ⋅ ρ(A)
= (⟦ba⟧(ρ))* ⋅ ρ(A)
= {ba}* ⋅ ρ(A)
= {ba}* ⋅ { (ba)ⁿb | n ∈ ℕ }
= { (ba)ᵏ | k ∈ ℕ } ⋅ { (ba)ⁿb | n ∈ ℕ }
= { (ba)ᵏ(ba)ⁿb | k, n ∈ ℕ }
= { (ba)ⁿb | n ∈ ℕ }
= ρ(S)
 
* Lösung zu Aufgabe 3.1.2
** Teilaufgabe a

#+include: "sol04-2a.c" src c

** Teilaufgabe b

#+include: "sol04-2b.c" src c

** Teilaufgabe c

#+include: "sol04-2c.c" src c

* Lösung zu Aufgabe 3.1.6

#+include: "sol04-3.c" src c
